Progress on connman proof

src/program_proof/memkv/connman_proof.v
@@ -11,7 +11,13 @@ Section connman_proof.
 Context `{!rpcregG Σ}.
 Context `{hG: !heapGS Σ}.
 Definition connmanN := nroot .@ "connman".
-Definition own_ConnMan (c_ptr:loc) : iProp Σ := True.
+Definition own_ConnMan (c_ptr:loc) : iProp Σ :=
+  ∃ (mref:loc) (rpcClsV:gmap u64 val) (rpcClsM:gmap u64 loc),
+    "HrpcCls" ∷ c_ptr ↦[ConnMan :: "rpcCls"] #mref ∗
+    "Hcls_map" ∷ map.is_map mref 1 (rpcClsV, zero_val (struct.ptrT rpc.RPCClient)) ∗
+    "#HownRpcCls" ∷ [∗ map] host ↦ cl;v ∈ rpcClsM;rpcClsV, RPCClient_own cl host ∗ ⌜v = #cl⌝
+.
+
 Definition is_ConnMan (c_ptr:loc) : iProp Σ :=
   ∃ mu,
   "#Hmu" ∷ readonly (c_ptr ↦[ConnMan :: "mu"] mu) ∗
@@ -46,12 +52,53 @@ Proof.
   wp_pures.
   wp_apply (wp_ref_of_zero).
   { done. }
-  iIntros (cl) "Hcl".
+  iIntros (cl_ptr) "Hcl_ptr".
   wp_pures.
   wp_loadField.
   wp_apply (acquire_spec with "Hinv").
   iIntros "[Hlocked Hown]".
   iNamed "Hown".
+  wp_pures.
+  wp_loadField.
+  wp_apply (map.wp_MapGet with "Hcls_map").
+  iIntros (cl1 ok1) "[%Hcl1 Hcls_map]".
+  wp_pures.
+  Search "wp_if".
+  wp_apply (wp_If_join (∃ (cl:loc), "Hown" ∷ own_ConnMan c_ptr ∗
+                        "Hcl" ∷ cl_ptr ↦[refT (struct.t rpc.RPCClient)] #cl ∗
+                        "#HisRpcCl" ∷ RPCClient_own cl host ∗
+                        "Hlocked" ∷ locked mu
+                       ) with "[-Hpre HΦ]"); first iSplit.
+  { (* *)
+    iIntros "HΦ".
+    (* TODO: apply spec for getNewClient *)
+    admit.
+  }
+  {
+    iIntros "[%Hnegb HΦ]".
+
+    destruct ok1 as [|] eqn:Hok; last first.
+    { exfalso. done. }
+    apply map.map_get_true in Hcl1.
+    iDestruct (big_sepM2_lookup_r with "HownRpcCls") as "HH".
+    { done. }
+    iDestruct "HH" as (cl) "[%Hcl [#HrpcCl %HclVal]]".
+
+    wp_apply (wp_StoreAt with "Hcl_ptr").
+    { naive_solver. }
+    iIntros "Hcl_ptr".
+    iApply "HΦ".
+
+    iExists cl.
+    rewrite HclVal.
+    iFrame "Hcl_ptr Hlocked #".
+    iExists _,_,_.
+    iFrame "∗#".
+  }
+  iNamed 1.
+  wp_pures.
+  wp_loadField.
+  wp_apply (release_spec with "[$Hinv $Hlocked $Hown]").
   wp_pures.
 Admitted.
 
